models/simlin/TPSimulationSet.v
@@ -17,70 +17,6 @@ Import LinCCALBase.
 Import LTSSpec.
 Import Semantics.
 
-Section AbstractConfig.
-  Context {F : Op.t} {VF : @LTS F}.
-
-  Definition AbstractConfigProp : Type := State VF -> tmap (@LinState F) -> Prop.
-
-  Record AbstractConfig : Type := mkAC {
-    ac_prop :> AbstractConfigProp;
-    ac_nonempty : exists ρ π, ac_prop ρ π;
-    ac_domexact : forall ρ1 π1 ρ2 π2, ac_prop ρ1 π1 -> ac_prop ρ2 π2 ->
-                    forall t, TMap.find t π1 = None <-> TMap.find t π2 = None
-  }.
-
-  Definition ac_equiv (Δ1 Δ2 : AbstractConfigProp) : Prop :=
-    forall ρ π, Δ1 ρ π <-> Δ2 ρ π.
-
-  Program Instance Equivalence_ACEquiv : Equivalence ac_equiv.
-  Next Obligation. constructor; auto. Defined.
-  Next Obligation. constructor; apply H. Defined.
-  Next Obligation.
-    constructor.
-    - unfold ac_equiv in *. intros. apply H0, H. auto.
-    - unfold ac_equiv in *. intros. apply H, H0. auto.
-  Defined.
-
-  Definition ac_subset (Δ1 Δ2 : AbstractConfigProp) : Prop :=
-    forall ρ π, Δ1 ρ π -> Δ2 ρ π.
-
-  Variant ac_singleton_prop ρ π : AbstractConfigProp :=
-  | ACSingle : ac_singleton_prop ρ π ρ π.
-
-  Program Definition ac_singleton ρ π : AbstractConfig :=
-    {| ac_prop := ac_singleton_prop ρ π |}.
-  Next Obligation. exists ρ, π. constructor. Qed.
-  Next Obligation.
-    inversion H; inversion H0; subst. reflexivity.
-  Qed.
-
-  Variant ac_union_prop (Δ1 Δ2 : AbstractConfigProp) : AbstractConfigProp :=
-  | ACUnionLeft ρ π: Δ1 ρ π -> ac_union_prop Δ1 Δ2 ρ π
-  | ACUnionRight ρ π: Δ2 ρ π -> ac_union_prop Δ1 Δ2 ρ π.
-
-  (* ac_union does not preserve ac_domexact in general *)
-  (* Program Definition ac_union (Δ1 Δ2 : AbstractConfig) : AbstractConfig := ... *)
-
-  Variant ac_intersect_prop (Δ1 Δ2 : AbstractConfigProp) : AbstractConfigProp :=
-  | ACIntersect ρ π: Δ1 ρ π -> Δ2 ρ π -> ac_intersect_prop Δ1 Δ2 ρ π.
-
-End AbstractConfig.
-
-Arguments AbstractConfigProp {F} VF.
-Arguments AbstractConfig {F} VF.
-
-#[global] Existing Instance Equivalence_ACEquiv.
-
-Delimit Scope ac_scope with AbstractConfig.
-Bind Scope ac_scope with AbstractConfig.
-
-Notation "[( ρ , π )]" := (ac_singleton ρ π) (at level 10) : ac_scope.
-Notation "Δ1 ⊆ Δ2" := (ac_subset Δ1 Δ2) (at level 70) : ac_scope.
-Notation "Δ1 ≡ Δ2" := (ac_equiv Δ1 Δ2) (at level 70) : ac_scope.
-Notation "Δ1 ∪ Δ2" := (ac_union_prop Δ1 Δ2) (at level 50) : ac_scope.
-Notation "Δ1 ∩ Δ2" := (ac_intersect_prop Δ1 Δ2) (at level 40) : ac_scope.
-
-
 (* threadpool simulation *)
 Module TPSimulation.
   Import Lang.
@@ -92,76 +28,8 @@ Module TPSimulation.
     Context {VF : @LTS F}.
     Context (M : ModuleImpl E F).
 
-    (* Definition AbstractConfig : Type := (@Poss F VF%type) -> Prop. *)
-    (* Definition AbstractConfig : Type := State VF -> tmap (@LinState F) -> Prop. *)
-
-    Variant ac_inv_prop (Δ : AbstractConfigProp VF) t f : AbstractConfigProp VF :=
-    | ACInv ρ π (Hposs : Δ ρ π) :
-        ac_inv_prop Δ t f ρ (TMap.add t (ls_inv f) π).
-
-    Program Definition ac_inv (Δ : AbstractConfig VF) t f : AbstractConfig VF :=
-      {| ac_prop := ac_inv_prop Δ t f |}.
-    Next Obligation.
-      destruct (ac_nonempty Δ) as [ρ [π H]].
-      exists ρ, (TMap.add t0 (ls_inv f) π). constructor. auto.
-    Qed.
-    Next Obligation.
-      inversion H; inversion H0; subst.
-      (* rewrite (ac_domexact Δ _ _ _ _ Hposs Hposs0 t0). *)
-      destruct (Pos.eq_dec t1 t0); subst.
-      - do 2 rewrite PositiveMap.gss. split; discriminate.
-      - do 2 (rewrite PositiveMap.gso; auto).
-        rewrite (ac_domexact Δ _ _ _ _ Hposs Hposs0 t1).
-        reflexivity.
-    Qed.
-
-    Variant ac_res_prop (Δ : AbstractConfigProp VF) t : AbstractConfigProp VF :=
-    | ACRes ρ π (Hposs : Δ ρ π):
-        ac_res_prop Δ t ρ (TMap.remove t π).
-    
-    Program Definition ac_res (Δ : AbstractConfig VF) t : AbstractConfig VF :=
-      {| ac_prop := ac_res_prop Δ t |}.
-    Next Obligation.
-      destruct (ac_nonempty Δ) as [ρ [π H]].
-      exists ρ, (TMap.remove t π). constructor. auto.
-    Qed.
-    Next Obligation.
-      inversion H; inversion H0; subst.
-      rewrite (ac_domexact Δ _ _ _ _ Hposs Hposs0 t0).
-      destruct (Pos.eq_dec t t0); subst.
-      - do 2 rewrite PositiveMap.grs. split; auto.
-      - do 2 (rewrite PositiveMap.gro; auto).
-        reflexivity.
-    Qed.
-
-    Variant ac_steps_prop (Δ : AbstractConfigProp VF) : AbstractConfigProp VF :=
-    | ACSteps ρ π ρ' π' (Hposs : Δ ρ π)
-        (Hpstep : poss_steps (PossOk ρ π) (PossOk ρ' π')):
-        ac_steps_prop Δ ρ' π'.
-
-    Lemma poss_steps_pi : forall ρ π ρ' π', poss_steps (PossOk ρ π) (PossOk ρ' π') -> π = π'.
-    Proof.
-      intros. remember (PossOk ρ π) as p. remember (PossOk ρ' π') as p'.
-      induction H; subst; auto.
-      inversion Heqp; subst.
-      (* We assume poss_step preserves pi. This depends on Semantics.v *)
-      admit.
-    Admitted.
-
-    Program Definition ac_steps (Δ : AbstractConfig VF) : AbstractConfig VF :=
-      {| ac_prop := ac_steps_prop Δ |}.
-    Next Obligation.
-      destruct (ac_nonempty Δ) as [ρ [π H]].
-      exists ρ, π. econstructor; eauto. apply rt_refl.
-    Qed.
-    Next Obligation.
-      inversion H; inversion H0; subst.
-      apply poss_steps_pi in Hpstep; apply poss_steps_pi in Hpstep0; subst.
-      eapply ac_domexact; eauto.
-    Qed.
-
     CoInductive TPSimulation (σ : State VE) (c : @ThreadPoolState E F) (Δ : AbstractConfig VF) : Prop :=
-    | TPSim_Error ρ π
+    | TPSim_Error (ρ : State VF) (π : LinCCALBase.tmap (@LinState F))
         (Hposs : Δ ρ π)
         (Herror : poss_steps (PossOk ρ π) (PossError)) :
         TPSimulation σ c Δ
@@ -191,15 +59,6 @@ Module TPSimulation.
 
     Definition cal (σ0 : State VE) (ρ0 : State VF) : Prop :=
       TPSimulation σ0 (TMap.empty _) (ac_init ρ0).
-
-    Open Scope ac_scope.
-
-    Lemma ac_steps_refl : forall Δ, Δ ⊆ ac_steps Δ.
-    Proof.
-      intros. intros ? ? ?.
-      econstructor; eauto.
-      apply rt_refl.
-    Qed.
 
     (* TODO: soundness: linearizability *)
   End Simulation.
